src/Cortex/Wire.hs
@@ -13,6 +13,8 @@ Wire modules own authoring and compilation mechanics while host authority stays 
 module Cortex.Wire
   ( module Cortex.Wire.Syntax
   , module Cortex.Wire.Circuit
+  , module Cortex.Wire.Circuit.Engine
+  , module Cortex.Wire.Circuit.Hosted
   , module Cortex.Wire.Executor
   , module Cortex.Wire.Include
   , module Cortex.Wire.Format
@@ -80,6 +82,8 @@ module Cortex.Wire
 where
 
 import Cortex.Wire.Circuit
+import Cortex.Wire.Circuit.Engine
+import Cortex.Wire.Circuit.Hosted
 import Cortex.Wire.Compile
   ( compileWireFile
   , compileWireFileWithEnv
